src/drf/PIStep.v
@@ -122,7 +122,8 @@ Proof.
     assert (STEPS' :=STEPS).
 
     generalize STEPT. intro STEPT'.
-    destruct cS, cT. inv STEPT. inv STEP; inv STEP0; ss.
+    destruct cS, cT. inv STEPT. guardH PFREE.
+    inv STEP; inv STEP0; ss.
     { subst. inv LOCAL. econs; eauto.
       - apply IdentMap.eq_leibniz.
         ii. setoid_rewrite IdentMap.map_add.
@@ -215,7 +216,8 @@ Proof.
               rewrite IdentMap.gso; eauto.
             }
     }
-    { inv STEPS. inv STEP; inv STEP0; try done. econs; eauto; ss.
+    { inv STEPS. des; [done|].
+      inv STEP; inv STEP0; try done. econs; eauto; ss.
       - apply IdentMap.eq_leibniz. ii.
         setoid_rewrite IdentMap.Properties.F.map_o in TID0.
         rewrite TID in TID0. inv TID0. depdes H1.
@@ -238,7 +240,8 @@ Proof.
           rewrite TID in TID1. inv TID1. eauto. }
         econs; eauto. rewrite IdentMap.gso; eauto.
     }
-    { inv STEPS. inv STEP; inv STEP0; try done. econs; eauto; ss.
+    { inv STEPS. des; [done|].
+      inv STEP; inv STEP0; try done. econs; eauto; ss.
       - apply IdentMap.eq_leibniz. ii.
         setoid_rewrite IdentMap.Properties.F.map_o in TID0.
         rewrite TID in TID0. inv TID0. depdes H1.
@@ -266,7 +269,8 @@ Proof.
           - eauto. }
         econs; eauto. rewrite IdentMap.gso; eauto.
     }
-    { inv STEPS. inv STEP; inv STEP0; try done. econs; eauto; ss.
+    { inv STEPS. des; [done|].
+      inv STEP; inv STEP0; try done. econs; eauto; ss.
       - apply IdentMap.eq_leibniz. ii.
         setoid_rewrite IdentMap.Properties.F.map_o in TID0.
         rewrite TID in TID0. inv TID0. depdes H1.
@@ -322,7 +326,8 @@ Proof.
           hexploit writing_small_step_fulfilled_new; try exact STEPS'; ss; eauto.
           i. inv H. esplits; eauto.
     }
-    { inv STEPS. inv STEP; inv STEP0; try done. econs; eauto; ss.
+    { inv STEPS. des; [done|].
+      inv STEP; inv STEP0; try done. econs; eauto; ss.
       - apply IdentMap.eq_leibniz. ii.
         setoid_rewrite IdentMap.Properties.F.map_o in TID0.
         rewrite TID in TID0. inv TID0. depdes H1.
@@ -378,7 +383,8 @@ Proof.
           hexploit writing_small_step_fulfilled_new; try exact STEPS'; ss; eauto.
           i. inv H. esplits; eauto.
     }
-    { inv STEPS. inv STEP; inv STEP0; try done. econs; eauto; ss.
+    { inv STEPS. des; [done|].
+      inv STEP; inv STEP0; try done. econs; eauto; ss.
       - apply IdentMap.eq_leibniz. ii.
         setoid_rewrite IdentMap.Properties.F.map_o in TID0.
         rewrite TID in TID0. inv TID0. depdes H1.
@@ -409,7 +415,8 @@ Proof.
           - eauto. }
         econs; eauto. rewrite IdentMap.gso; eauto.
     }
-    { inv STEPS. inv STEP; inv STEP0; try done. econs; eauto; ss.
+    { inv STEPS. des; [done|].
+      inv STEP; inv STEP0; try done. econs; eauto; ss.
       - apply IdentMap.eq_leibniz. ii.
         setoid_rewrite IdentMap.Properties.F.map_o in TID0.
         rewrite TID in TID0. inv TID0. depdes H1.
@@ -582,7 +589,7 @@ Lemma small_step_is_promised
   Threads.is_promised x l t c2.(Configuration.threads).
 Proof.
   inv PROMISED. destruct msg.
-  inv STEP. ss.
+  inv STEP. guardH PFREE. ss.
   destruct (Ident.eq_dec x tid); cycle 1.
   { econs; eauto. rewrite IdentMap.gso; eauto. }
   subst. rewrite TID in TID0. inv TID0. apply inj_pair2 in H1. subst.
@@ -608,7 +615,8 @@ Proof.
   inv PSTEPS1. inv USTEP. revert STEPS. condtac; cycle 1.
   { i. destruct cST3. esplits; cycle 1.
     - econs 2; eauto. econs; eauto. econs. econs; eauto.
-      + inv STEPS. inv STEPT. econs; eauto.
+      + inv STEPS. des; [done|]. destruct pf; ss. inv STEPT. clear PFREE0. econs; eauto.
+        destruct pf; eauto. inv STEP0; ss. inv STEP1; ss.
       + rewrite COND. ss.
     - ss.
     - omega.
@@ -623,15 +631,15 @@ Proof.
     - omega.
   }
   inversion A12. inv PI_STEP. inv USTEP.
-  assert (E0: ThreadEvent.is_promising e0 = None); [by inv STEPT0|].
+  destruct (ThreadEvent.is_promising e0) as [[]|] eqn:E0.
+  { admit. }
   destruct p.
   exploit reorder_promise_small_step; try exact STEPT; eauto.
   { inv WF. auto. }
-  { rewrite E0 in *. ii.
-    hexploit pi_wf_small_step_is_reading; try exact WF2; eauto. i.
+  { ii. hexploit pi_wf_small_step_is_reading; try exact WF2; eauto. i.
     hexploit pi_wf_small_step_is_promising; eauto.
   }
-  { apply rtcn_rtc in A23.
+  { apply rtcn_rtc in A23. inv A12.
     exploit pi_step_except_small_step; eauto. i. destruct cST3. ss.
     exploit pi_step_future; try exact WF2; eauto. i. des. inv WF0.
     clear -CONSIS WFT x0.
@@ -642,14 +650,17 @@ Proof.
   }
   i. des. unguardH STEP2. des.
   { destruct cST3. inv STEP2. esplits; cycle 1.
-    - econs 2; eauto. econs; eauto. econs. econs; eauto.
-      ii. eapply NOWR0; eauto.
-      eapply small_step_is_promised; eauto.
+    - econs 2; eauto. econs; eauto. econs.
+      econs; eauto.
+      + rewrite E0. ss.
+      + ii. eapply NOWR0; eauto.
+        eapply small_step_is_promised; eauto.
     - ss.
     - omega.
   }
   assert (STEP1': pi_step_evt false tid0 (cS2, cT1) (cS0, c1')).
   { econs; eauto. econs; eauto.
+    - rewrite E0. ss.
     - etrans; eauto. inv STEP0. s. rewrite IdentMap.Facts.add_o. condtac; ss.
       subst. inv STEP; [|by inv STEP0; inv PROMISING]. inv STEP0. ss. inv PROMISING.
       rewrite TID0. eauto.
@@ -660,9 +671,10 @@ Proof.
   { econs. econs; eauto.
     - rewrite PROMISING. ss.
     - destruct (Ident.eq_dec tid0 tid); subst; ss.
-      rewrite E0 in *.
-      inv STEPS. s. rewrite IdentMap.gso; auto.
-      inv STEPT0. s. rewrite IdentMap.gso; auto.
+      admit.
+      (* rewrite E0 in *. *)
+      (* inv STEPS. s. rewrite IdentMap.gso; auto. *)
+      (* inv STEPT0. s. rewrite IdentMap.gso; auto. *)
     - ii. destruct e1'; ss.
   }
   exploit IH; try exact STEP2'; eauto.
@@ -671,7 +683,7 @@ Proof.
   - econs; eauto.
   - ss.
   - omega.
-Qed.
+Admitted.
 
 Lemma rtc_pi_step_remove_promises_aux
       tid tidex cST1 cST2 cST3
